coq/Frontend/SQL/SQL.v
@@ -1,0 +1,124 @@
+(*
+ * Copyright 2015-2016 IBM Corporation
+ *
+ * Licensed under the Apache License, Version 2.0 (the "License");
+ * you may not use this file except in compliance with the License.
+ * You may obtain a copy of the License at
+ *
+ * http://www.apache.org/licenses/LICENSE-2.0
+ *
+ * Unless required by applicable law or agreed to in writing, software
+ * distributed under the License is distributed on an "AS IS" BASIS,
+ * WITHOUT WARRANTIES OR CONDITIONS OF ANY KIND, either express or implied.
+ * See the License for the specific language governing permissions and
+ * limitations under the License.
+ *)
+
+(****************
+ * SQL mini-BNF *
+ ****************
+
+// From inspecting the TPC-H queries
+
+Query ::= "select" SelectExpr ("," SelectExpr)*
+          "from" FromExpr ("," FromExpr)*
+          ( "where" Cond )?
+	  ( "group by" GroupExpr ("," GroupExpr)*
+	    ( "having" Cond )? )?                          /* having only allowed for group by */
+	  ( "order by" SortCriteria ("," SortCriteria)* )?
+	  
+SelectExpr ::= Column | Expr "as" Column
+
+Agg ::= "sum" | "avg" | "count"
+
+FromExpr ::= Column | "(" Query ")" "as" TableSpec
+
+Condition ::= Condition ("and" | "or") Condition
+      |  "not" Condition
+      |  Expr ("=" | "<=" | "<" | ">" | ">=" | "<>") Expr
+      |  "exists" "(" Query ")"
+      |  Expr "in" Expr
+      |  Expr "not" "in" Expr
+      |  Expr "like" Expr
+      |  Expr "between" Expr "and" Expr
+
+GroupExpr ::= Column
+
+SortCriteria ::= Column ("asc" | "desc")?
+
+Expr ::= Constant
+      |  Column
+      |  "*"
+      |  Expr ("-" | "+" | "*" | "/") Expr
+      |  Agg "(" Expr ")"
+      |  Agg "(" Query ")"
+
+Constant ::= INT | FLOAT | STRING | "date" STRING
+          |  "(" Constant ("," Constant)* ")
+
+TableSpec ::= TableName ( "(" Column ("," Column)* ")" )?
+Column ::= IDENT
+TableName ::= IDENT
+
+Note: Do we want to support 'case' (q12) -- seems relatively big an extension
+Note: Do we want to support 'substring' (q22) -- seems just meh...
+Note: Do we want to support 'create view' (q15) -- seems relatively trivial through environments
+"
+*)
+
+Section SQL.
+
+  Require Import String.
+  Require Import List.
+  Require Import Arith.
+  Require Import EquivDec.
+
+  Require Import Utils BasicSystem.
+
+  Context {fruntime:foreign_runtime}.
+
+  Definition sql_env := list (string * data).
+
+  Unset Elimination Schemes.
+
+  Require Import RDataSort.
+  (* TableSpec ::= TableName "(" Column, ("," Column)* ")" )? *)
+  Definition table_spec : Set := string * (option (list string)).
+  Definition order_spec : Set := SortCriterias.
+
+  Inductive sql_query : Set :=
+  | SQuery :
+      list sql_select ->                                 (* Select Clause *)
+      list sql_from ->                                   (* From Clause *)
+      option sql_condition ->                            (* Where Clause *)
+      option ((list string) * (option sql_condition)) -> (* GroupBy Clause *)
+      option SortCriterias -> sql_query                  (* OrderBy Clause *)
+  with sql_select : Set :=
+  | SSelectColumn : string -> sql_select
+  | SSelectExpr : string -> sql_expr -> sql_select
+  with sql_from : Set :=
+  | SFromColumn : string -> sql_from
+  | SFromQuery : table_spec -> sql_query -> sql_from
+  with sql_condition : Set :=
+  | SCondAnd : sql_condition -> sql_condition -> sql_condition
+  | SCondOr : sql_condition -> sql_condition -> sql_condition
+  | SCondNot : sql_condition -> sql_condition
+  | SCondExists : sql_query -> sql_condition
+  | SCondIn : sql_expr -> sql_expr -> sql_condition
+  with sql_expr : Set :=
+  | SExprConst : data -> sql_expr
+  | SExprColumn : string -> sql_expr
+  | SExprStar : sql_expr
+  | SExprBinop : binOp -> sql_expr -> sql_expr -> sql_expr
+  | SExprAggExpr : unaryOp -> sql_expr -> sql_expr (* Has to be an aggregate unaryOp! *)
+  | SExprAggQuery : unaryOp -> sql_query -> sql_expr (* Has to be an aggregate unaryOp! *)
+  .
+
+  
+End SQL.
+
+(* 
+*** Local Variables: ***
+*** coq-load-path: (("../../../coq" "QCert")) ***
+*** End: ***
+*)
